Tests/Meta/SpecAndSimp.lean
@@ -1,12 +1,45 @@
 import HouLean.Meta.SpecializeAndSimp.Main
+import HouLean.OpenCL.Basic
+import HouLean.OpenCL.Reference.Operators
+import HouLean.Data.Matrix
+import HouLean.Data.Vector
+-- import HouLean.OpenCL.Data.Matrix
+
 import Qq
 
 open Lean Meta Qq HouLean Meta
 
-def foo (x : Nat) :=
+open OpenCL.Compiler2
+def skipImplementedBy (e : Expr) : MetaM Bool := do
+  let s := (compilerExt.getState (← getEnv)).implementedBy
+  let candidates ← s.getMatch e
+  for c in candidates do
+    let (xs,_,_) ← forallMetaTelescope (← inferType c.lhs)
+    let b := c.lhs.beta xs
+    if ← isDefEq e b then
+      let mut skip := false
+      for x in xs do
+        let t ← inferType x
+        if (← isClass? t).isSome then
+          if (← synthInstance? t).isNone then
+            skip := true
+      if skip then
+        continue
+      logInfo m!"skipping specialization of {e}"
+      return true
+  return false
+
+
+def foo {α} [Add α] [Mul α] (x : α) :=
   let a := x*x
   let b := x+x
   a + b + x
+
+-- set_option trace.Meta.Tactic.simp true
+set_option trace.HouLean.specialize true
+#eval foo 10
+
+attribute [opencl_csimp] Nat.add_zero Nat.zero_add
 
 run_meta
   let e :=
@@ -17,11 +50,40 @@ run_meta
         a1 * a2
       let b :=
         let b1 := y + 3
-        let b2 := 0 + foo a + 0
+        let b2 := 0 + foo a + 0 + foo 10
         b1 * a * b2
       a + b)
 
   lambdaTelescope e fun _ e => do
-  let e' ← specializeAndSimp e {} { zeta := false } #[`simp]
+  let e' ← specializeAndSimp e {} { zeta := false } #[`opencl_csimp] skipImplementedBy
+
+  logInfo e'
+
+
+impl_by (x y z : Float) : #v[x,y,z] ==> (float3){x,y,z}
+
+impl_by {α : Type} (u : Vector α 3) (h : 0 < 3) : getElem u 0 h ==> u.x
+impl_by {α : Type} (u : Vector α 3) (h : 1 < 3) : u[1]'h ==> u.y
+impl_by {α : Type} (u : Vector α 3) (h : 2 < 3) : u[2]'h ==> u.z
+
+@[opencl_csimp]
+theorem vector_map (v : Vector α n) (f : α → β) : v.map f = .ofFn (fun i => f v[i]) := sorry_proof
+
+@[opencl_csimp]
+theorem vector_ofFn (f : Fin 3 → α) : Vector.ofFn f = #v[f 0, f 1, f 2] := sorry_proof
+
+
+-- variable (x : Vector Float 3)
+-- #check (Vector.map Math.sin x) rewrite_by
+macro_rules | `(tactic| get_elem_tactic_extensible) => `(tactic| sorry_proof)
+
+
+set_option trace.HouLean.specialize.detail true
+run_meta
+  let e :=
+    q(fun x y z : Float => #v[x,y,z])
+
+  lambdaTelescope e fun _ e => do
+  let e' ← specializeAndSimp e {} { zeta := false } #[`opencl_csimp] skipImplementedBy
 
   logInfo e'
